Compiler/CompilationModel/LogicalPurity.lean
@@ -50,7 +50,7 @@ partial def exprContainsCallLike (expr : Expr) : Bool :=
   | Expr.adtField _ _ _ _ _ =>
       false
   | Expr.literal _ | Expr.param _ | Expr.constructorArg _ | Expr.storage _ | Expr.storageAddr _
-  | Expr.caller | Expr.contractAddress | Expr.chainid | Expr.msgValue | Expr.blockTimestamp
+  | Expr.caller | Expr.contractAddress | Expr.chainid | Expr.msgValue | Expr.selfBalance | Expr.blockTimestamp
   | Expr.blockNumber | Expr.blobbasefee
   | Expr.calldatasize | Expr.returndataSize | Expr.localVar _ | Expr.arrayLength _ | Expr.storageArrayLength _
   | Expr.adtTag _ _ =>
@@ -141,7 +141,7 @@ def exprContainsUnsafeLogicalCallLike (expr : Expr) : Bool :=
   | Expr.adtField _ _ _ _ _ =>
       false
   | Expr.literal _ | Expr.param _ | Expr.constructorArg _ | Expr.storage _ | Expr.storageAddr _
-  | Expr.caller | Expr.contractAddress | Expr.chainid | Expr.msgValue | Expr.blockTimestamp
+  | Expr.caller | Expr.contractAddress | Expr.chainid | Expr.msgValue | Expr.selfBalance | Expr.blockTimestamp
   | Expr.blockNumber | Expr.blobbasefee
   | Expr.calldatasize | Expr.returndataSize | Expr.localVar _ | Expr.arrayLength _ | Expr.storageArrayLength _
   | Expr.adtTag _ _ =>
